chore(data/finset): remove has_choice class, improve proofs

data/option.lean
@@ -118,12 +118,11 @@ instance lift_or_get_idem (f : α → α → α) [h : is_idempotent α f] :
   is_idempotent (option α) (lift_or_get f) :=
 ⟨λ a, by cases a; simp [lift_or_get, h.idempotent]⟩
 
-instance lift_or_get_choice (f : α → α → α) [has_choice f] : has_choice (lift_or_get f) :=
-⟨λ o₁ o₂, match o₁, o₂ with
-| none  , none   := or.inl rfl
-| some a, none   := or.inl rfl
-| none  , some b := or.inr rfl
-| some a, some b := by simpa [lift_or_get] using choice f a b
-end⟩
+theorem lift_or_get_choice {f : α → α → α} (h : ∀ a b, f a b = a ∨ f a b = b) :
+  ∀ o₁ o₂, lift_or_get f o₁ o₂ = o₁ ∨ lift_or_get f o₁ o₂ = o₂
+| none     none     := or.inl rfl
+| (some a) none     := or.inl rfl
+| none     (some b) := or.inr rfl
+| (some a) (some b) := by simpa [lift_or_get] using h a b
 
 end option
