logic/basic.lean
@@ -625,17 +625,14 @@ end nonempty
 
 /- binary choice functions -/
 
-class has_choice {α : Sort*} (f : α → α → α) : Prop :=
-(choice : ∀ a b, f a b = a ∨ f a b = b)
+theorem if_choice {α : Sort*} (c : Prop) [decidable c] (a b : α) :
+  ite c a b = a ∨ ite c a b = b :=
+by by_cases h : c; simp [h]
 
-def choice {α : Sort*} (f : α → α → α) [has_choice f] : ∀ (a b : α), f a b = a ∨ f a b = b :=
-has_choice.choice f
+theorem min_choice {α : Type*} [decidable_linear_order α] (a b : α) :
+  min a b = a ∨ min a b = b :=
+by by_cases h : a ≤ b; simp [min, h]
 
-instance if_choice {α : Sort*} (c : Prop) [d : decidable c] : has_choice (@ite c d α) :=
-⟨λ a b, by by_cases h : c; simp [h]⟩
-
-instance min_choice {α : Sort*} [d : decidable_linear_order α] : has_choice (@min α d) :=
-⟨λ a b, by simp [min, (if_choice (a ≤ b)).choice]⟩
-
-instance max_choice {α : Sort*} [d : decidable_linear_order α] : has_choice (@max α d) :=
-⟨λ a b, if h : a ≤ b then or.inr (max_eq_right h) else or.inl (max_eq_left_of_lt (lt_of_not_ge h))⟩
+theorem max_choice {α : Type*} [decidable_linear_order α] (a b : α) :
+  max a b = a ∨ max a b = b :=
+by by_cases h : a ≤ b; simp [max, h]
